code/rocq/valid_state.v
@@ -3,7 +3,7 @@ From det Require Import lang.
 
 Module valid_state (U:Unif).
   Module Run := Run(U).
-  Include Run.
+  Import Run.
   
   Fixpoint base_and s :=
     match s with
@@ -11,6 +11,9 @@ Module valid_state (U:Unif).
     | Top => true
     | _ => false
     end.
+
+  Lemma base_and_dead {A}: base_and (dead A) = false.
+  Proof. case: A => // -[]//=. Qed.
 
   Fixpoint base_or_aux s :=
     match s with
@@ -25,9 +28,9 @@ Module valid_state (U:Unif).
     | _ => false
     end.
 
-  Fixpoint base_and_ko s :=
+  Definition base_and_ko s :=
     match s with
-    | And KO r r1 => [&&base_and r, (cut r == r1) & base_and_ko r1] (* should also say something about the program *)
+    | And KO r r1 => [&&base_and r, (r == r1) & base_and r1] (* should also say something about the program *)
     | KO => true
     | _ => false
     end.
@@ -38,36 +41,59 @@ Module valid_state (U:Unif).
     | t => base_and_ko t
     end.
 
+  Lemma base_and_big_and {pr A}: base_and (big_and pr A).
+  Proof. by elim: A => // a l /= ->; rewrite eq_refl. Qed.
+
   (* same_structure_and *)
   Section ssa.
     Fixpoint ssa A B :=
       match A, B with
       | And _ _ _, Or _ _ _ => false
-      | And _ _ _, Dead => true
       | And _ _ A, And _ _ B => ssa A B
-      | Top, (Top|OK|KO) => true
+      | Top, (Top|OK|KO|Dead) => true
       | _, _ => false
       end.
+
+    Lemma xxx {B C D}: base_and B -> base_and D -> ssa B C -> ssa D C -> ssa B D.
+    Proof.
+      elim: B C D => //.
+      + move=>[]//[]//=[]//.
+      + move=> []//p a _ A HA B HB[]//=C D E []//.
+        move=> []///= _ _ F G.
+        move=>/andP[]/eqP <- bA /andP[]/eqP? ssA ssF.
+        apply: HA => //.
+    Qed.
+
+
     Lemma ssa_id {A}: base_and A -> ssa A A.
     Proof. by elim: A =>// -[]// p a _ B0 HB0 B HB/=/andP[] _. Qed.
 
     Lemma ssa_cut {A}: base_and A -> ssa A (cut A).
-    Proof. by elim: A =>// -[]// p a _ B0 HB0 B HB/=/andP[] _. Qed.
+    Proof. elim: A =>// -[]// p a _ B0 HB0 B HB/=/andP[] _; apply ssa_id. Qed.
+
+    Lemma ssa_dead {A}: base_and A -> ssa A (dead A).
+    Proof. elim: A =>//= -[]// p a _ B0 HB0 B HB/=/andP[] _//; apply ssa_id. Qed.
 
     Lemma ssa_cut1 {A B}: ssa A B -> ssa A (cut B).
     Proof.
-      elim: A B => //.
-        move=> []//.
-      move=> A HA B0 _ B HB[]//.
+      elim: A B; try by move=> // [] //.
+      - move=> A HA B0 _ B HB[]//.
+    Qed.
+
+    Lemma ssa_dead1 {A B}: ssa A B -> ssa A (dead B).
+    Proof.
+      elim: A B; try by move=> // [] //.
+      - move=> A HA B0 _ B HB[]//.
     Qed.
 
     Lemma ssa_cut2 {A B}: base_and B -> ssa A (cut B) -> ssa A B.
     Proof.
-      elim: A B => //.
-        move=> []//.
-      move=> A HA B0 _ B HB[]//[]//.
-      move=> p a s1 s2/=/andP[]/eqP?;subst.
-      apply: HB.
+      elim: A B; try by move=> []//.
+      (* - move=> /= _ _ []//.
+      - move=> A HA s B HB []//. *)
+      - move=> A HA B0 _ B HB[]//[]//.
+        (* move=> p a s1 s2/=/andP[]/eqP?;subst.
+        apply: HB. *)
     Qed.
 
     (* Lemma xxx {B C D}: ssa B C -> ssa D C -> ssa B D.
@@ -84,60 +110,78 @@ Module valid_state (U:Unif).
         - move=> ? _ _ [] <-//.
         - move=> ?? _ _ [] <-//<-//.
         - move=> ?? _ _ [] <-//<-//.
-      move=> []// p a _ A HA B0 HB0 []//A' B0' B' s.
-        move=>/=<-//.
-      move=> r /= /andP[/eqP <-] bA ssA.
-      case: r.
+        - move=> ? _ _ [] <-//.
+      move=> []// p a _ A HA B0 HB0 []// A' B0' B' s.
+      move=>/= r /andP[]/eqP? bB ssB0;subst.
+      case: r =>//.
       + move=> s1 C /simpl_expand_and_expanded[].
           move=>[A2[HA' ->]]//.
         move=>[s' [A2 [B2 [HA' [HB' ->]]]]]//=.
-        apply: HA _ _ _ bA ssA HB'.
+        by apply: HA _ _ _ bB _ HB'.
       + move=> s1 C /simpl_expand_and_cut[].
           move=>[A2 [HA' ->]]//.
         move=> [s'[A2[B2 [HA'[HB' ->]]]]]/=.
-        apply: HA _ _ _ bA ssA HB'.
+        by apply: HA _ _ _ bB _ HB'.
       + move=> C /simpl_expand_and_fail[].
-          move=> [HA' ->]//=.
-        move=>[].
-          move=> [A2 [DA[HA' ->]]]//.
-        move=> [s'[A2[B2[HA'[HB' ->]]]]]/=.
-        case: ifP => ///eqP H .
-        by rewrite (HA _ _ _ bA ssA HB').
+          move=> [A2 [HA' ->]]//=.
+        move=>[s' [A2[B2 [HA' [HB' ->]]]]]//=.
+        by rewrite (HA _ _ _ bB ssB0 HB').
       + move=> s1 C /simpl_expand_and_solved.
-        move=> [s'[A1[B1[HA'[HB' <-]]]]]/=.
-        by have /= := (HA _ _ _ bA ssA HB').
+        move=> [s'[A1[B1[HA'[HB' ->]]]]]/=.
+        by have /= := (HA _ _ _ bB ssB0 HB').
     Qed.
   End ssa.
 
-  
+  Lemma base_or_dead {B}: base_or_aux B || base_or_aux_ko B -> B <> dead B.
+  Proof.
+    move=>/orP[].
+      elim: B => //.
+        move=> A HA s B HB /=/andP [bA bB][dA dB].
+        by move: bA; rewrite dA; rewrite base_and_dead.
+      move=> []//.
+    elim: B => //.
+      move=> A HA s B HB /=/andP[bA bB] [dA dB].
+      apply: HB; auto.
+    move=>[]//.
+  Qed.
+
+
   Fixpoint valid_state s :=
     match s with
     | Goal _ _ | OK | KO | Bot | Top => true
     | Dead => false
-    | Or Dead _ r => valid_state r
-    | Or l _ r => valid_state l && (base_or_aux r || base_or_aux_ko r)
-    | And l r0 r => 
-      [&& valid_state l, 
-        if success l then valid_state r else ((r0 == r) || (cut r0 == r)),
-        ssa r0 r &
-        (base_and r0)]
+    | Or A _ B => 
+      if A == dead A then valid_state B
+      else valid_state A && (base_or_aux B || base_or_aux_ko B)
+    | And A B0 B => 
+      [&& valid_state A,
+        if success A then valid_state B 
+        else (B0 == B)
+        (* ssa B0 B & *)
+        & (base_and B0)]
     end.
+
+  Lemma valid_state_dead {A} : valid_state (dead A) = false.
+  Proof.
+    elim: A => //.
+      by move=> A HA s B HB/=; rewrite dead_dead_same eqxx.
+    move=> A HA Bo ? B HB/=.
+    rewrite HA//.
+  Qed.
 
   Lemma base_and_valid {A} : base_and A -> valid_state A.
   Proof.
     elim A => //; clear => A HA B +; rewrite /base_or_aux //=; case: A HA => //.
     move=> p a _ + A + /andP [] /eqP H ; rewrite H.
     move=> _ HVA HA; rewrite (HVA HA) /=.
-    by rewrite HA eq_refl (ssa_id HA).
+    by rewrite HA eq_refl ?(ssa_id HA).
   Qed.
 
-  Lemma base_and_big_and {pr A}: base_and (big_and pr A).
-  Proof. by elim: A => // a l /= ->; rewrite eq_refl. Qed.
 
   Lemma valid_state_big_and {pr l} : valid_state (big_and pr l).
   Proof.
     elim: l => // x xs /=.
-    by rewrite base_and_big_and eq_refl/= (ssa_id base_and_big_and).
+    by rewrite base_and_big_and eq_refl/= ?(ssa_id base_and_big_and).
   Qed.
 
   Lemma base_or_big_and {pr l} : base_or_aux (big_and pr l).
@@ -153,34 +197,20 @@ Module valid_state (U:Unif).
   Lemma base_or_valid {A} : base_or_aux A -> valid_state A.
   Proof.
     elim A => //; clear.
-    + move=> A HA s B HB/=/andP[]/base_and_valid->/[dup]/HB->->; destruct A => //.
-    + by move=> []// p a Ha B0 HB0 B HB /=/andP[/eqP->]bB; rewrite eqxx bB (ssa_id bB).
+    + move=> A HA s B HB/=/andP[bA bB].
+      case:ifP => /eqP.
+        by move=>H; move: bA; rewrite H base_and_dead.
+      rewrite bB // base_and_valid//.
+    + move=> []// p a Ha B0 HB0 B HB /=/andP[/eqP->]bB.
+      by rewrite eqxx bB ?(ssa_id bB).
   Qed.
 
-  Lemma dead_big_or p s t: big_or p s t <> dead (big_or p s t).
-  Proof.
-    rewrite /big_or; case F: F => // [[s1 r] xs] //.
-  Qed.
-
-  Lemma simpl_valid_state_or {s A B}: valid_state (Or A s B) -> (A = Dead /\ valid_state B) \/ (A <> Dead /\ valid_state A /\ (base_or_aux B || base_or_aux_ko B)).
-  Proof.
-    move=> /=; case: A => //.
-    all: try by move=> /= ->; right; repeat split => //; rewrite orbT //.
-    + move=> /= ->; left => //.
-    + move=> ?? /orP [] ->; right; repeat split => //; rewrite orbT //.
-    + move=> ??? /andP [] H ->; right => //.
-    + move=> ??? /andP [] H ->; right => //.
-  Qed.
 
   Lemma base_and_ko_valid {B}: base_and_ko B -> valid_state B.
   Proof.
     elim: B => //.
-    by move=> []// HA B0 _ B HB/=/and3P[bB0 /eqP <-]; rewrite bB0 eqxx orbT (ssa_cut bB0).
+    move=> []// HA B0 _ B HB/=/and3P[bB0 /eqP <-] H; rewrite bB0 eqxx ?(ssa_id bB0)//.
   Qed.
-
-  Lemma simpl_valid_state_and1 {A B0 B}: valid_state (And A B0 B) -> 
-    valid_state A /\ (if success A then valid_state B else (B0 == B) || (cut B0 == B)) /\ ssa B0 B /\ base_and B0.
-  Proof. by move=>/=/and3P[]//->->/andP[]->->. Qed.
 
 
   Lemma base_or_ko_valid {B}: base_or_aux_ko B -> valid_state B.
@@ -188,8 +218,9 @@ Module valid_state (U:Unif).
     elim: B => //.
     + move=> A HA s B HB /= /andP [] /base_and_ko_valid ->.
       move=> /[dup] /HB -> ->.
-      by rewrite !orbT; destruct A.
-    + by move=> [] // HA B0 _ B HB /= /and3P[] bB0 /eqP <-; rewrite eq_refl bB0 orbT (ssa_cut bB0).
+      by rewrite orbT if_same.
+    + move=> [] // HA B0 _ B HB /= /and3P[] bB0 /eqP <-.
+      by rewrite eq_refl bB0 ?(ssa_id bB0).
   Qed.
 
 
@@ -198,11 +229,49 @@ Module valid_state (U:Unif).
   Proof. by move=> /orP []; [move=> /base_or_valid | move=> /base_or_ko_valid] => ->. Qed.
 
 
+  Lemma simpl_valid_state_or {s A B}: 
+    valid_state (Or A s B) -> 
+      (A = dead A /\ valid_state B) \/ 
+      (A <> dead A /\ valid_state A /\ (base_or_aux B || base_or_aux_ko B)).
+  Proof.
+    move=> /=; case: A => //.
+    all: try by move=> /= ->; right; repeat split => //; rewrite orbT //.
+    + move=> /= ->; left => //.
+    + move=> ?? /orP [] ->; right; repeat split => //; rewrite orbT //.
+    + move=> ???; case:ifP=>/eqP//.
+        by move=>/=[]->->; rewrite !dead_dead_same eqxx; left.
+      move=> H/andP[]->->; auto.
+    + move=> ???; case:ifP=>/eqP.
+        move=>->->; rewrite dead_dead_same; auto.
+      move=>? /andP[]->->; auto.
+  Qed.
+
+  Lemma simpl_valid_state_or1 {s A B}: 
+    valid_state (Or A s B) -> 
+      (A = dead A /\ valid_state B) \/ 
+      (A <> dead A /\ valid_state A /\ valid_state B).
+  Proof.
+    move=> /simpl_valid_state_or[]; auto.
+    move=> [?[?/base_or_base_or_ko_valid]]; auto.
+  Qed.
+
+
+  Lemma simpl_valid_state_and1 {A B0 B}: valid_state (And A B0 B) -> 
+    valid_state A /\ 
+      ( 
+        (* if A == dead A then B == dead B else  *)
+        if success A then valid_state B 
+        else ((B0 == B) )) 
+      /\ (*ssa B0 B /\*) base_and B0.
+  Proof. by move=>/=/and3P[]//->->/andP[]->->. Qed.
+
+
+
   Lemma base_and_base_and_ko_cut {B} : base_and B -> base_and_ko (cut B).
   Proof. 
     elim: B => // A + B + C /=.
     case: A => //= _ _ _ HB HC /andP [] /eqP <- hB.
-    by rewrite hB (HB hB) eqxx.
+    by rewrite hB eqxx.
   Qed.
 
   Lemma base_or_base_or_ko_cut {B}: base_or_aux B -> base_or_aux_ko (cut B).
@@ -210,14 +279,14 @@ Module valid_state (U:Unif).
     elim: B => //.
     + by move=> A IHA s B IHB /= /andP [] /base_and_base_and_ko_cut -> /IHB ->.
     + move=> [] //= _ _ _ B HB C HC /andP [] /eqP /[subst1] hC.
-      by rewrite eq_refl hC (base_and_base_and_ko_cut hC). 
+      by rewrite eq_refl hC ?(base_and_base_and_ko_cut hC). 
   Qed.
 
   Lemma base_and_ko_cut {B}: base_and_ko B -> base_and_ko (cut B).
   Proof.
     elim: B => //.
     move=> []// _ B _ C HC /= /and3P[] bB /eqP <-.
-    by rewrite cut_cut_same eqxx bB => ->.
+    (* by rewrite cut_cut_same eqxx bB => ->. *)
   Qed.
   
   Lemma base_or_ko_cut {B}: base_or_aux_ko B -> base_or_aux_ko (cut B).
@@ -225,77 +294,57 @@ Module valid_state (U:Unif).
     elim: B => //.
       by move=> A HA s B HB /= /andP[]/base_and_ko_cut->/HB->.
     move=> [] //= _ B0 _ B HB /and3P[] bB /eqP<-.
-    by rewrite cut_cut_same bB eqxx => ->.
+    (* by rewrite cut_cut_same bB eqxx => ->. *)
   Qed.
-
-  Lemma cut_dead1 {A}: cut A = dead A -> A = dead A.
-  Proof. by elim: A=> // A HA s B HB[]/=/HA<-/HB<-. Qed.
 
   Lemma success_cut {A} : success (cut A) = success A.
   Proof.
     elim: A => //. 
     + move=> A HA s B HB /=.
       rewrite dead_cut_is_dead.
-      case: eqP.
-        move=> /cut_dead1//.
-        move=>->; rewrite dead_dead_same eq_refl//.
+      case:ifP=>/eqP.
+        by move=> /cut_dead1//->; rewrite eqxx.
       by case: eqP => //->; rewrite dead_dead_same cut_dead_is_dead.
     + move=> A HA B HB C HC /=.
-      by rewrite HA HC.
+      by rewrite HA ?HC.
   Qed.
 
   Lemma valid_state_cut {A}: valid_state A -> valid_state (cut A).
   Proof.
     elim: A => //.
       move=> A HA s B HB/simpl_valid_state_or[].
-        by move=>[]->/=.
+        by move=>[]/=->; rewrite cut_dead_is_dead dead_dead_same eqxx.
       move=> [DA[VA bB]]/=.
       rewrite (HA VA) (HB (base_or_base_or_ko_valid bB)).
-      move: bB => /orP[/base_or_base_or_ko_cut | /base_or_ko_cut]->; rewrite orbT; destruct A => //.
-    move=> A HA B0 _ B HB /=/simpl_valid_state_and1[VA [+ [ssaB0 bB0]]].
+      by move: bB => /orP[/base_or_base_or_ko_cut | /base_or_ko_cut]->; rewrite !orbT if_same.
+    move=> A HA B0 _ B HB /=/simpl_valid_state_and1[VA [+ bB0]].
     rewrite (HA VA) success_cut bB0 andbT/=.
-    case: ifP => //.
-      move=>// _ VB. rewrite (HB VB) ssa_cut1//.
-    move=> _/orP[].
-      move=>/eqP?;subst; rewrite eqxx orbT (ssa_cut)//.
-    move=>/eqP<-; rewrite cut_cut_same eqxx orbT ssa_cut//.
+    case: ifP => sA.
+      (* move=>->/eqP->; rewrite !cut_dead_is_dead !dead_dead_same !eqxx ssa_dead1//. *)
+    (* move=> dA; case: ifP => sA. *)
+      move=>vB; rewrite vB//?ssa_cut1//.
+    move=> /eqP<-; rewrite eqxx ?ssa_id//.
   Qed.
 
   Lemma valid_state_compose_and {A2 B2 B02}: 
-    (if success A2 then valid_state B2 else ((B02 == B2) || (cut B02 == B2))) ->
+    (if success A2 then valid_state B2 else ((B02 == B2))) ->
       base_and B02  ->
         valid_state B2.
   Proof. 
     case: success => //.
-      move=>/orP[].
-        move=>/eqP->; apply: base_and_valid.
-      move=>/eqP<-/base_and_valid.
-      apply: valid_state_cut.  
+    (* move=>/orP[]. *)
+      move=>/eqP->; apply: base_and_valid.
+    (* move=>/eqP<-/base_and_valid;apply: valid_state_cut. *)
   Qed.
-  (* Lemma base_and_base_and_ko_valid {B}:
-    base_and B || base_and_ko B -> valid_state B.
-  Proof. by move=> /orP []; [move=> /base_and_valid | move=> /base_and_ko_valid] => ->. Qed. *)
-
-
 
   Lemma simpl_valid_state_and {A B0 B}: valid_state (And A B0 B) -> 
     valid_state A /\ valid_state B.
   Proof.
-    move=>/= /and3P[]//=> ->; case:success => ///orP[]/eqP<-/andP[] _.
-      move=>/base_and_valid//.
-    by move=>/base_and_valid /valid_state_cut->.
+    move=>/= /and3P[]// -> VB bbB0.
+    by rewrite (valid_state_compose_and VB bbB0).
   Qed.
 
-
-  Lemma valid_state_is_not_dead A: valid_state A -> A <> dead A.
-  Proof. 
-    elim: A => //.
-    move=> A HA s B HB /simpl_valid_state_or[].
-      move=> [] -> /HB + []//.
-    move=>[]+[]/HA++[]//.
-  Qed.
-
-  Lemma expand_failure_dead s1 {A}: valid_state A -> expand s1 A <> Failure Dead.
+  (* Lemma expand_failure_dead s1 {A}: valid_state A -> expand s1 A <> Failure Dead.
   Proof.
     elim: A s1 => //.
     + move=> /= p [] //.
@@ -315,10 +364,7 @@ Module valid_state (U:Unif).
       move=> []s'[]A'[]B'[]H1[]H2.
       case: eqP => ///[subst1].
       by have:= HB s' VB.
-    Qed.
-
-  Lemma success_dead {A}: success (dead A) = false.
-  Proof. by elim: A=> // A HA s B HB /=; rewrite HA HB if_same. Qed.
+    Qed. *)
 
   Lemma valid_state_big_or {pr s t} : valid_state (big_or pr s t).
   Proof.
@@ -326,286 +372,210 @@ Module valid_state (U:Unif).
     + by move=> ?; case: F => //= -[] //=???; rewrite base_or_big_or_aux.
     + by move=> ?; case: F => //= -[] //=???; rewrite base_or_big_or_aux.
     + by move=> ??; case F => //= -[] //=???; rewrite base_or_big_or_aux.
-  Qed. 
-
-  
+  Qed.   
 
   Lemma expand_not_dead {s A r}: 
-    valid_state A -> expand s A = r -> get_state r <> dead (get_state r).
+    valid_state A -> expand s A = r -> get_state r <> dead (get_state r) .
   Proof.
     elim: A s r; try by move=> //= _ r _ <-//.
-    + by move=> p [|t] s r _ <- //=; apply dead_big_or.
+    + move=> p [|t] s r _ <- //= /esym; apply dead_big_or.
     + move=> A HA s B HB s1 => // C /simpl_valid_state_or [].
         move=> []->/= VB <-.
+        rewrite dead_dead_same eqxx.
         have {}HB:= HB _ _ VB.
         case X: expand => //=; have:= HB _ _ X => /=; try congruence.
-        by move=> H; case: ifP => /eqP H1; subst => //= -[]//.
+        (* by move=> H; case: ifP => /eqP H1; subst => //= -[]//. *)
       move=> [DA[VA VB]].
       case: C.
       + move=> s2 C /simpl_expand_or_expanded [].
-          by move=> [A'[+]] /[subst1] /HA => /(_ VA) /=; congruence.
+          move=> [A'[DA'[HA' ->]]]/=[].
+          by have /= := HA _ _ VA HA'.
         move=> [].
-          by move=> [A'[]] /HA => /(_ VA)/= HA' -> /=; rewrite dead_cut_is_dead; congruence.
-        move=> [H [B']] []-> []/HB => /(_ (base_or_base_or_ko_valid VB))/=; try congruence.
+          move=> [A'[dA []]] /HA => /(_ VA)/= HA' -> /=; rewrite dead_cut_is_dead; congruence.
+        move=>  [->[B' [H]]]->/=.
+        rewrite dead_dead_same => -[].
+        by move: H => []/HB/=/(_ (base_or_base_or_ko_valid VB))//.
       + move=> s2 C /simpl_expand_or_cut [s3[B'[?]]]; subst => //.
       + move=> C /simpl_expand_or_fail[].
-          move=>[A'[HA'[DA']]]->/=.
+          move=>[A'[dA[HA']]]/=->.
           have:= HA _ _ VA HA' => /=; congruence.
-        move=>[].
-          move=> [B'[DB'[HA'[HB']]]] -> /=; have:= HB _ _ (base_or_base_or_ko_valid VB) HB' => /=; congruence.
-        move=> [HA'[HB' DD]].
-        by have:= HA _ _ VA HA'.
+        by move=>[B'[X]]; move: VA; rewrite X valid_state_dead.
       + move=> s2 C /simpl_expand_or_solved [].
           move=> [A'[]] /HA{} => /(_ VA) /= H ->/=; congruence.
         move=> [B'[HA'[]]] /HB => /(_ (base_or_base_or_ko_valid VB)) /= + ->/=; congruence.
     + move=> A HA B0 HB0 B HB s1 r /simpl_valid_state_and[] VA VB.
       case: r.
       + move=> s2 C /simpl_expand_and_expanded [].
-          by move=> [A'][] /HA H1 -> //.
-        move=> [s'[A'[B'[]]]] /HA /= +[] _ ->//.
+          by move=> [A'][] /HA => /(_ VA) /= ? ->[].
+        by move=> [s'[A'[B'[]]]] /HA /= +[] _ ->//= => /(_ VA) + [].
       + move=> s2 C /simpl_expand_and_cut [].
-          move=> [A'][] /HA /= + ->//.
-        move=> [s'[A'[B'[]]]] /HA/= + [] _->//.
+          by move=> [A'][] /HA /= + ->// => /(_ VA) + [].
+        move=> [s'[A'[B'[]]]] /HA/= + [] _->// => /(_ VA) + [].
+        rewrite dead_cut_is_dead => H /cut_dead1; congruence.
       + move=> C /simpl_expand_and_fail [].
-          move=> [] H; have:= HA _ _ VA H => //.
-        move=>[].
-          by move=> [A'[DA[]]] /= + ->//.
-        move=> [s'[A'[B'[HA' [HB']]]]]->/=.
-        by case: ifP => /eqP?;subst => //; have:= HB _ _ VB HB'.
-      + move=> s2 C /simpl_expand_and_solved [s'[A'[B']]] [].
-        by move=>/= + []/HB/= + <-.
+          by move=>[A'[H ->]]/=[]; have:= (HA _ _ VA H).
+        move=>[s'[A'[B'[HA'[HB' ->]]]]]/=[].
+        by have:= HA _ _ VA HA'.
+      + move=> s2 C /simpl_expand_and_solved [s'[A'[B'[HA'[HB'->]]]]]/=[].
+        by have:= HA _ _ VA HA'.
   Qed.
 
-  Lemma valid_state_dead {A}: valid_state (dead A) = false.
-  Proof. by elim: A => // A HA s B HB/=; rewrite HA HB; case: dead. Qed.
+  (* Lemma expand_failure_dead *)
 
   Lemma succes_is_solved s {A}: valid_state A -> success A -> exists B, expand s A = Solved s B.
   Proof.
     elim: A s => //; try by do 2 eexists.
-    + move=> A HA s1 B HB s /=.
-      case: ifP => /eqP.
-      + move=> ->; rewrite valid_state_dead; case X: (dead A) => // H1 H2 /=.
-        have [C H]:= HB s H1 H2.
-        by eexists; rewrite H => //.
-      + move=> DA H.
-        have {H}: (valid_state A && (base_or_aux B || base_or_aux_ko B)).
-          destruct A => //.
-        move=>/andP[]VA VB SA.
-        have [A' H]:= HA s VA SA.
-        by rewrite H; eexists.
+    + move=> A HA s1 B HB s /simpl_valid_state_or[].
+        move=>[-> vB]/=.
+        rewrite dead_dead_same eqxx.
+        move=>sB.
+        by have [B' H] := HB s vB sB; rewrite H; eexists.
+      move=>[dA[vA bB]]/=.
+      case:ifP => /eqP// _ sA.
+      by have [A' H] := HA s vA sA; rewrite H; eexists.
     + move=> A HA B0 HB0 B HB s /simpl_valid_state_and[] VA VB /=/andP[SA SB].
       have [A' H1]:= HA s VA SA; rewrite H1.
       have [B' H2]:= HB s VB SB; rewrite H2.
       by eexists.
-  Qed. 
-
-  Lemma expand_solved_failed {s1 A s2 B}: valid_state A -> expand s1 A = Solved s2 B -> failed A = false /\ failed B = false.
-  Proof.
-    elim: A s1 s2 B => //.
-    + by move=> ???? [] /[subst2]; repeat split.
-    + move=> ?[]//.
-    + move=> A HA s B HB s1 s2 C /simpl_valid_state_or[].
-        move=> []->/=/HB{}HB; case X: expand => //= -[] _ <-/=; apply: HB X.
-      move=> [] H []/[dup]VA/HA{}HA/base_or_base_or_ko_valid/HB{}HB/simpl_expand_or_solved [].
-      + move=> [A'[+]] /[subst1] /=/[dup] /HA []->-> /(expand_not_dead VA) /=.
-        repeat case: eqP => //.
-        by move: VA => + DA H1; rewrite H1 valid_state_dead.
-      + move=> [A'[]]/= + [] /HB[] /= -> + -> /= => + ->.
-        by have:= expand_failure_dead s1 VA.
-    + move=> A HA B0 _ B HB s1 s2 C + /simpl_expand_and_solved [s3 [A' [B' ]]][]/HA{}HA[]/HB{}HB.
-      move=> /simpl_valid_state_and[]VA VB <-/=.
-      have:= HA VA => -[]->->.
-      have:= HB VB => -[]->->.
-      do 2 case: success => //.
   Qed.
 
-  Lemma expand_solved_success {s1 A s2 B}: valid_state A -> expand s1 A = Solved s2 B -> success A /\ success B.
+  Lemma expand_solved_success {s1 A s2 B}: 
+    valid_state A -> expand s1 A = Solved s2 B -> success A /\ success B.
   Proof.
     elim: A s1 s2 B => //.
     + by move=> /= ???? [] /[subst2].
     + move=> ? [] //.
     + move=> A HA s B HB s1 s2 C /simpl_valid_state_or[].
-        move=> [] -> /=/HB{}HB; case X: expand => //= -[] _ <-; move: X => /HB //.
-      move=> []H[]/[dup] VA/HA{}HA/[dup]BB/base_or_base_or_ko_valid/HB{}HB/simpl_expand_or_solved [].
-        move=> [A'] [] +  /[subst1] /[dup] + /HA[] /=->-> => /(expand_not_dead VA)/=; do 2 case: eqP =>//.
-        by move: VA => + _ H1; rewrite H1 valid_state_dead.
-      move=> [B'[H1]].
-      by have:= expand_failure_dead s1 VA.
+        move=> [] -> vB/=.
+        rewrite dead_dead_same eqxx.
+        case X: expand => //=-[]*;subst => /=.
+        rewrite dead_dead_same eqxx.
+        apply: HB X => //.
+      move=> [dA[VA bB]] /simpl_expand_or_solved[].
+        move=>[A'[HA' ->]]/=.
+        have:= expand_not_dead VA HA' => /=.
+        do 2 case: ifP => /eqP //; try congruence.
+        move=> ???; apply: HA VA HA'.
+      move=> [B'[]]//.
     + move=> A HA ? _ B HB s1 s2 C /simpl_valid_state_and[VA VB].
-      move=> /simpl_expand_and_solved [s3 [A' [B'[HA' [HB' <-]]]]]/=.
+      move=> /simpl_expand_and_solved [s3 [A' [B'[HA' [HB' ->]]]]]/=.
       have:= HA _ _ _ VA HA' => -[] ->->.
       by have:= HB _ _ _ VB HB' => -[] ->->.
   Qed.
 
-  Lemma expand_failure_not_dead_right {s1 A B}: valid_state A -> expand s1 A = Failure B -> (A <> dead A) -> (B <> dead B).
+  Lemma expand_solved_failed {s1 A s2 B}: 
+    valid_state A -> expand s1 A = Solved s2 B -> failed A = false /\ failed B = false.
   Proof.
-    elim: A B s1 => //.
-    + by move=> ??? [] /[subst1] //.
-    + by move=> ? [] //.
-    + move=> A HA s B HB C s1 /simpl_valid_state_or [].
-        move=> []->/[dup]VB /HB{}HB/=.
-        case X: expand => // [D]-[] <-.
-        move: X => /HB H H1.
-        have {H1}: B <> dead B.
-          move=> HH; apply: H1 => []; congruence.
-        move=> /H; case: eqP.
-          move=> ->//.
-        move=> /= _ H2 []; auto.
-      move=> []DA[]/[dup]/HA{}HA VA /base_or_base_or_ko_valid /[dup] VB /HB{}HB /simpl_expand_or_fail [].
-        move=> [A'[]]/[dup]HH/HA{}HA[] H1-> /= H2 [] H3 H4.
-        by move: VB; rewrite H4; rewrite valid_state_dead.
-      move=> [].
-        move=> [B'[+]] [] /HA{}HA[]/HB{}HB/=->/= + [] H.
-        have: B <> dead B.
-          by move=> H1; move: VB; rewrite H1 valid_state_dead.
-        by move=> /HB.
-      move=> []/HA {}HA; 
-      have: A <> dead A.
-        move: VA => + H; rewrite H valid_state_dead//.
-      move=> /HA//.
-    + move=> A HA B0 HB0 B HB C s1 /simpl_valid_state_and[] VA VB /simpl_expand_and_fail [].
-        move=> [] /HA{}HA.
-        have: A <> dead A.
-          by move: VA => + H; rewrite H valid_state_dead//.
-        move=> /HA []//.
-      move=> [].
-        move=> [A'[DA[HA']]] -> //.
-      move=> [s'[A'[B'[HA' [HB' ->]]]]]/= _.
-      have H1 := HB _ _ VB HB'.
-      case: ifP => ///eqP/[subst1].
-      have: B <> dead B.
-        move: VB => + H; rewrite H valid_state_dead//.
-      by move=>/H1.
+    move=>/expand_solved_success H /H[].
+    by do 2 move=> /success_failed->.
   Qed.
-
 
   Lemma expand_failure_failed {s1 A B}:
     valid_state A -> expand s1 A = Failure B -> failed A /\ failed B.
   Proof.
     elim: A s1 B; clear => //; try by move=> ? [] //.
     + move=> A HA s1 B HB s2 C /simpl_valid_state_or[].
-        move=> [] ->/=; case X: expand => //= /HB{}HB [] <-; move: X=>/HB[]->.
-        by case: eqP => //.
+        move=> [] ->/=; rewrite dead_dead_same eqxx.
+        case X: expand => //= /HB{}HB [] <-; move: X=>/HB[]->/=.
+        by rewrite dead_dead_same eqxx.
       move=> [DA] [] /[dup] VA /HA{}HA/[dup]BB/base_or_base_or_ko_valid/HB{}HB/simpl_expand_or_fail [].
-        move=> [A' [+[HD]]] /[subst1] /= => /[dup].
-        move=> /HA [] -> ->; move: VA; case: eqP.
-          by move=> ->; rewrite valid_state_dead.
-        move=> /expand_failure_not_dead_right{}HA/HA{}HA/HA.
-        by case: eqP => //.
-      move=>[].
-        move=> [B'[HD[+[+]]]]  /[subst1] /=.
-        by move=> /HA [] -> _ /HB [] -> ->; rewrite if_same.
-      by move=> [+[+]] /[subst1] /= => /HA [] -> _ /HB [] -> _; rewrite if_same.
+        move=> [A' [+[HD]]] /[subst1] /= dA.
+        have /= dA' :=expand_not_dead VA HD.
+        do 2 case: ifP => /eqP//; try congruence.
+        move=> _ _.
+        apply: HA HD.
+      move=> [B'[dA[HB'->]]]; rewrite dA /=.
+      rewrite dead_dead_same eqxx.
+      by apply: HB HB'.
     + move=> A HA B0 _ B HB s C/simpl_valid_state_and[VA VB].
       move=> /simpl_expand_and_fail[].
-        move=> [] HA' ->/=.
-        by have:= HA _ _ VA HA'=>-[]-> //.
-      move=> [].
-        move=> [A'[DA'[HA' ->]]]/=.
-        by have:= HA _ _ VA HA' => -[]->->.
+        move=> [A' [HA'->]]/=.
+        by have:= HA _ _ VA HA'=>-[]-> //->.
       move=> [s' [A' [B' [HA' [HB' ->]]]]]/=.
-      have:= HB _ _ VB HB' => -[].
-      have:= expand_solved_success VA HA' => -[] ->.
-      case: ifP.
-        by move=>/eqP -> _ ->; rewrite orbT.
-      by move=> _ /= ->->->; rewrite !orbT.
+      have:= HB _ _ VB HB' => -[]->->.
+      have:= expand_solved_success VA HA' => -[] ->->.
+      by rewrite !orbT.
   Qed. 
 
 
   Lemma valid_state_expand {s A r}:
-    expand s A = r -> valid_state A -> valid_state (get_state r).
+    valid_state A -> expand s A = r -> valid_state (get_state r).
   Proof.
-    elim: A s r => //; try by move=> s r // /[subst1] //.
-    + by move=> ? [|?] ?? /[subst1] //=; rewrite valid_state_big_or.
-    + move=> A IHA s B IHB s1 [s2 C|||].
-      + move=> /simpl_expand_or_expanded [|[]].
-        + move=> [A'[HA']] /[subst1] /simpl_valid_state_or [].
-          + move=> [] /[subst1] //.
-          + move=> [] _ [] VA /[dup] /base_or_base_or_ko_valid /= -> ->; rewrite (IHA _ _ HA' VA); destruct A' => //.
-        + move=> [A'[HA']] /[subst1] /simpl_valid_state_or [].
-          + move=> [] /[subst1] //.
-          + move=> [] _ [] VA /[dup] /base_or_base_or_ko_valid /= VB BB.
-            suffices:  valid_state A' && (base_or_aux (cut B) || base_or_aux_ko (cut B)).
-              destruct A' => //.
-            by move: BB; rewrite (IHA _ _ HA' VA) => /orP [/base_or_base_or_ko_cut|/base_or_ko_cut] ->; rewrite orbT.
-        + move=> [] HA [B' +] /simpl_valid_state_or [] [] DA => -[] /[subst1] H /=.
-          + by move: H => [] /IHB {}IHB /IHB ->.
-          + by move: H => [] /IHB {}IHB [] _ /base_or_base_or_ko_valid /IHB //.
-      + move=> s2 C /simpl_expand_or_cut [s3[B'[?[HB]]]] /[subst1] /simpl_valid_state_or [].
-        + move=> [] _ VB; apply: IHB HB VB.
-        + move=> []//.
-      + move=> C /simpl_expand_or_fail [|[]].
-        + move=> [A'[HA'[DA']]] /[subst1] /simpl_valid_state_or[] [].
-          + move=> /[subst1]; simpl in HA'; congruence.
-          + move=> DA [] VA /[dup] /base_or_base_or_ko_valid /= -> ->; rewrite (IHA _ _ HA' VA); destruct A' => //.
-        + move=> [B'[DB'[HA'[HB']]]] /[subst1] /simpl_valid_state_or [] [].
-          + by move=> ? VB /[subst] /=; rewrite (IHB _ _ HB' VB).
-          + by move=> ? [] VA /base_or_base_or_ko_valid /(IHB _ _ HB') /= ->.
-        + move=> [HA'[HB']] /[subst1] /simpl_valid_state_or [][].
-          + move=> /[subst1] /(IHB _ _ HB') //.
-          + move=> DA [VA] /base_or_base_or_ko_valid.
-            by move=> /(IHB _ _ HB').
-          + move=> s2 C /simpl_expand_or_solved [].
-            + move=> [A'[HA']] /[subst1] /simpl_valid_state_or [] [].
-              + move=> /[subst1] //.
-              + by move=> DA [VA] /= /[dup] /base_or_base_or_ko_valid -> ->; rewrite (IHA _ _ HA' VA); destruct A' => //.
-            + move=> [B'[HA'[HB']]] /[subst1] /simpl_valid_state_or [][].
-              + by move=> /[subst1] VB /=; rewrite (IHB _ _ HB' VB).
-              + by move=> DA [] VA /base_or_base_or_ko_valid /= VB; rewrite (IHB _ _ HB' VB).
-    + move=> A HA B0 _ B HB s1 [].
+    elim: A s r => //; try by move=> s r // *; subst.
+    + by move=> ? [|?] ?? *;subst => //=; rewrite valid_state_big_or.
+    + move=> A IHA s B IHB s1 r /simpl_valid_state_or[].  
+        move=> []->VB/=; rewrite dead_dead_same eqxx.
+        case X: expand => *; subst => /= ; rewrite dead_dead_same eqxx;
+        by have:= IHB _ _ VB X.
+      move=> [dA [VA bB]].
+      case: r.
+      + move=> s2 C /simpl_expand_or_expanded [].
+          move=> [A'[_[HA' ->]]]/=.
+          rewrite (IHA _ _ VA HA') bB.
+          have /= dA':= expand_not_dead VA HA'.
+          case: ifP => // _.
+          by apply: base_or_base_or_ko_valid.
+        move=> [].
+          move=>[A'[_[HA' ->]]]/=.
+          have/=->:= IHA _ _ VA HA'.
+          rewrite (valid_state_cut (base_or_base_or_ko_valid bB)).
+          by move: bB => /orP[/base_or_base_or_ko_cut|/base_or_ko_cut]->; rewrite orbT if_same.
+        move=>[]//.
+      + move=> s2 C /simpl_expand_or_cut. 
+        move=> [s3[B'[dA'[HB]]]]//.
+      + move=> C /simpl_expand_or_fail [].
+          move=>[A'[_[HA'->]]]/=.
+          have /= dA':= expand_not_dead VA HA'.
+          by case: ifP => /eqP// _; rewrite bB (IHA _ _ VA HA').
+        move=>[B'[?]]//.
+      + move=> s2 C /simpl_expand_or_solved [].
+          move=> [A'[HA' ->]]/=.
+          have /= dA':= expand_not_dead VA HA'.
+          by case: ifP => /eqP//; rewrite bB (IHA _ _ VA HA').
+        move=> [B'[?]]//.
+    + move=> A HA B0 _ B HB s1 r /simpl_valid_state_and1[VA[VB bB0]].
+      case: r.
       + move=> s2 C => /simpl_expand_and_expanded [].
-          move=> [A'[HA' ->]] /simpl_valid_state_and1 [VA [VB [ssaB0 bB0]]]/=.
-          rewrite (HA _ _ HA' VA) bB0 (valid_state_compose_and VB bB0) ssaB0.
-          move: VB; case SA: success.
-            have:= succes_is_solved s1 VA SA; rewrite HA' => -[?] //.
+          move=> [A'[HA' ->]]/=.
+          rewrite (HA _ _ VA HA') bB0 (valid_state_compose_and VB bB0) ?ssB0.
+          move: VB.
+          case: ifP => //sA.
+          have:= succes_is_solved s1 VA sA; rewrite HA' => -[?] //.
           by move=>->; rewrite if_same.
-        move=> [s[A'[B'[HA'[HB' ->]]]]].
-        move=> /simpl_valid_state_and1 [VA].
-        have:= expand_solved_success VA HA' => -[]/=->-> [VB [ssaB0 bB0]].
-        by rewrite (HA _ _ HA' VA) (HB _ _ HB' VB)  bB0 (ssa_expand bB0 ssaB0 HB').
+        move=> [s[A'[B'[HA'[HB' ->]]]]]/=.
+        have:= expand_solved_success VA HA' => -[] _ ->.
+        rewrite (HA _ _ VA HA') (HB _ _ (valid_state_compose_and VB bB0) HB') bB0.
+        by rewrite ?(ssa_expand bB0 ssB0 HB').
       + move=> s2 C /simpl_expand_and_cut [].
-          move=> [A' [HA' ->]] /simpl_valid_state_and1[VA [VB [ssaB0 bB0]]]/=.
-          rewrite (HA _ _ HA' VA) bB0 (valid_state_compose_and VB bB0).
+          move=> [A' [HA' ->]]/=.
+          rewrite (HA _ _ VA HA') bB0 (valid_state_compose_and VB bB0).
           move: VB; case SA: success.
             have:= succes_is_solved s1 VA SA; rewrite HA' => -[?] //.
-          by move=>->; rewrite if_same ssaB0.
-        move=> [s'[A'[B'[HA'[HB' ->]]]]]/simpl_valid_state_and1[VA [VB [ssaB0 bB0]]]/=.
+          by move=>->; rewrite if_same ?ssB0.
+        move=> [s'[A'[B'[HA'[HB' ->]]]]]/=.
         move: VB.
         have:= expand_solved_success VA HA' => -[] -> sA' VB.
-        rewrite (HB _ _ HB' VB) success_cut bB0 sA' (valid_state_cut (HA _ _ HA' VA)).
-        by rewrite (ssa_expand bB0 ssaB0 HB').
+        rewrite (HB _ _ VB HB') success_cut bB0 sA' (valid_state_cut (HA _ _ VA HA')).
+        by rewrite ?(ssa_expand bB0 ssB0 HB').
       + move=> s2 /simpl_expand_and_fail [].
-          by move=> [] /expand_failure_dead H _ /simpl_valid_state_and1 [] /H.
-        move=> [].
-          move=> [A'[DA'[HA' ->]]] /simpl_valid_state_and1 [VA[VB [ssaB0 bB0]]] /=.
-          rewrite (HA _ _ HA' VA) bB0 ssaB0.
-          move: VB.
-          have:= expand_failure_failed VA HA' => -[].
-          do 2 move=> /failed_success->.
-          by move=>->.
-        move=> [s'[A'[B'[HA'[HB' ->]]]]] /simpl_valid_state_and1 [VA [VB [ssaB0 bB0]]]/=.
-        have:= HA _ _ HA' VA.
-        have:= HB _ _ HB' (valid_state_compose_and VB bB0).
-        move=>/=.
-        case: ifP => [/eqP->|]// _ /=->->.
+          move=>[A'[HA'->]]/=.
+          rewrite (HA _ _ VA HA') bB0 ?ssB0.
+          have []:= expand_failure_failed VA HA'.
+          move: VB; case: ifP => //sA ->.
+            by move=> /failed_success; rewrite sA.
+          case: ifP => //.
+          by move=>/success_failed ->.
+        move=> [s'[A'[B'[HA'[HB' ->]]]]]/=.
+        have:= HA _ _ VA HA'.
+        have:= HB _ _ (valid_state_compose_and VB bB0) HB' => /=.
+        move=>->->.
         have:= expand_solved_success VA HA' => -[] _ ->.
-        by rewrite (ssa_expand bB0 ssaB0 HB') bB0.
-      + move=> s C /simpl_expand_and_solved [s'[A'[B'[HA' [HB'<-]]]]].
-        move=> /simpl_valid_state_and1 [VA [+ [ssaB0 bB0]]].
-        have:= expand_solved_success VA HA' => /= -[] ->-> VB.
-        rewrite (HA _ _ HA' VA) (HB _ _ HB' VB) bB0.
-        by rewrite (ssa_expand bB0 ssaB0 HB').
-  Qed.
-
-  Lemma expand_failure_not_dead_left {s1 A B}: valid_state A -> expand s1 A = Failure B -> B <> Dead -> A <> dead A.
-  Proof.
-    elim: A B => //.
-    + move=> A HA s B HB C VA /simpl_expand_or_fail [|[]].
-      + move=> [A'[HA'[?]]] /[subst1] /= H -[] H1 H2.
-        by move: VA; rewrite H1 H2; rewrite (@valid_state_dead (Or A s B)).
-      + move=> [B'[?[HA'[HB']]]] /[subst1] /= H [] H1 H2.
-        by move: VA; rewrite H1 H2; rewrite (@valid_state_dead (Or A s B)).
-      + move=> [+[]] => //.
+        by rewrite ?(ssa_expand bB0 ssB0 HB') bB0.
+      + move=> s C /simpl_expand_and_solved [s'[A'[B'[HA' [HB'->]]]]]/=.
+        move: VB.
+        have:= expand_solved_success VA HA' => -[]->-> VB.
+        rewrite (HA _ _ VA HA') (HB _ _ VB HB') bB0.
+        by rewrite ?(ssa_expand bB0 ssB0 HB').
   Qed.
 
   Lemma valid_state_big_or_aux {pr s l} : valid_state (big_or_aux pr s l).
@@ -613,7 +583,7 @@ Module valid_state (U:Unif).
     elim: l s => [|[]] //=.
     + move=> s; rewrite valid_state_big_and // full_expanded_big_and.
     + move=> _ r l IH s.
-      rewrite valid_state_big_and base_or_big_or_aux IH; case: big_and => //.
+      by rewrite valid_state_big_and base_or_big_or_aux IH /= if_same.
   Qed.
 
   Lemma toT {P}: P = true -> is_true P.
@@ -626,14 +596,14 @@ Module valid_state (U:Unif).
   Proof.
     move=> + [b H]; elim H; clear.
     + move=> s1 s2 A1 A2 EA VA /=.
-      apply: valid_state_expand EA VA.
+      apply: valid_state_expand VA EA.
     + move=> s A B HA HB /=.
-      apply: valid_state_expand HA HB.
+      apply: valid_state_expand HB HA.
     + move=> s s' r A B b HA HB IH VA.
-      have VB:= valid_state_expand HA VA.
+      have VB:= valid_state_expand VA HA.
       apply: IH VB.
     + move=> s s' r A B b HA HB IH VA.
-      have VB:= valid_state_expand HA VA.
+      have VB:= valid_state_expand VA HA.
       apply: (IH VB).
   Qed.
 
@@ -642,81 +612,55 @@ Module valid_state (U:Unif).
   Proof.
     move=> + [b H].
     elim: H; clear.
-    + move=> s1 s2 A B HA VA /=; apply: valid_state_expand HA VA.
-    + move=> s A B HA VA; apply: valid_state_expand HA VA.
-    + move=> s1 s2 r A B b HA _ IH VA; apply (IH (valid_state_expand HA VA)).
-    + move=> s1 s2 r A B b HA _ IH VA; apply (IH (valid_state_expand HA VA)).
+    + move=> s1 s2 A B HA VA /=; apply: valid_state_expand VA HA.
+    + move=> s A B HA VA; apply: valid_state_expand VA HA.
+    + move=> s1 s2 r A B b HA _ IH VA; apply (IH (valid_state_expand VA HA)).
+    + move=> s1 s2 r A B b HA _ IH VA; apply (IH (valid_state_expand VA HA)).
   Qed.
 
-  Lemma next_alt_aux_base_and {s1 s2 A B}:
-     base_and A || base_and_ko A ->  next_alt_aux true s1 A = Some (s2, B) -> A = B.
+  (* Lemma next_alt_aux_base_and {s1 s2 A B}:
+     base_and A || base_and_ko A ->  next_alt s1 A = Some (s2, B) -> A = B.
   Proof.
     elim: A s1 s2 B => //; move=> [] //.
     + move=> _ B0 _ B HB s1 s2 C /= /and3P[] bB0 /eqP cB0 bcB0.
-      case NB: next_alt_aux => // [[ ]] [] /[subst2].
+      case NB: next_alt => // [[ ]] [] /[subst2].
       by have:= HB _ _ _ _ NB; rewrite bcB0 orbT => /(_ isT) <-.
     + move=> p a _ B0 HB0 B HB s1 s2 C /= /orP []// /andP []/eqP/[subst1] BB.
-      case NB: next_alt_aux => // [[ ]] [] /[subst2].
+      case NB: next_alt => // [[ ]] [] /[subst2].
       by rewrite BB in HB; rewrite (HB _ _ _ isT NB).
+  Qed. *)
+
+  Lemma next_alt_aux_base_and1 {A s}: base_and A -> next_alt s A = None.
+  Proof.
+    elim: A s => //-[]//p a _ B0 _ B HB/= c.
+    move=>/andP[]/eqP? bB;subst.
+    by rewrite HB.
   Qed.
 
-  Lemma next_alt_aux_base_and1 {s1 s2 A B}:
-     base_and A ->  next_alt_aux true s1 A = Some (s2, B) -> A = B.
+  Lemma next_alt_aux_base_and2 {A s}: base_and A -> next_alt s (cut A) = None.
   Proof.
-    elim: A s1 s2 B => //; move=> [] //.
-    + move=> p a _ B0 HB0 B HB s1 s2 C /= /andP []/eqP/[subst1] BB.
-      case NB: next_alt_aux => // [[ ]] [] /[subst2].
-      by rewrite BB in HB; rewrite (HB _ _ _ isT NB).
+    elim: A s => //-[]//p a _ B0 _ B HB/= c.
+    (* move=>/andP[]/eqP? bB;subst.
+    rewrite next_alt_aux_base_and1//. *)
   Qed.
 
-  Lemma next_alt_aux_base_and2 {s1 s2 A B}:
-     base_and A ->  next_alt_aux true s1 (cut A) = Some (s2, B) -> cut A = B.
-  Proof.
-    elim: A s1 s2 B => //; move=> [] //.
-    + move=> p a _ B0 HB0 B HB s1 s2 C /= /andP []/eqP/[subst1] BB.
-      case NB: next_alt_aux => // [[ ]] [] /[subst2].
-      by rewrite BB in HB; rewrite (HB _ _ _ isT NB).
-  Qed.
-
-  (* Lemma xx {A B s}:
-    base_and A ->ssa A B -> 
-      exists s', next_alt_aux false s B = Some (s', A).
-  Proof.
-    elim: A B s => //.
-      move=>/= []//=. *)
-
-    Lemma xxx {B C D}: base_and B -> base_and D -> ssa B C -> ssa D C -> ssa B D.
-    Proof.
-      elim: B C D => //.
-      + move=>[]//[]//.
-      + move=> []//p a _ A HA B HB[]//.
-          move=>/= + /andP[/eqP? bB] + _; subst.
-          move=>[]//=[]//.
-          move=> _ _ C D/andP[]/eqP? bD _; subst.
-          admit.
-        move=> A1 A2 A3 []//.
-        move=> []// p1 a1 A5 A6 /=/andP[]/eqP? bB; subst.
-        move=>/andP[]/eqP? bA6 ssaB ssaA6; subst.
-        by apply: HA ssaA6.
-    Admitted.
-
-
-  Lemma ssa_next_alt_aux {B0 B s1 s2 D b}: 
+  (* Lemma ssa_next_alt_aux {B0 B s1 s2 D}: 
     base_and B0 -> ssa B0 B -> valid_state B ->
       (* valid_state B -> *)
-        next_alt_aux b s1 B = Some (s2, D) -> ssa B0 D.
+        next_alt s1 B = Some (s2, D) -> ssa B0 D.
   Proof.
-    elim: B0 B s1 s2 D b => //.
+    elim: B0 B s1 s2 D => //.
       by move=> []//= s1 s2 D []// _ _ _ []??;subst.
     move=>[]//p A IGN /= B0 HB0 B HB.
-    move=>[]// A' B0' B' s1 s2 D b.
+    move=>[]// A' B0' B' s1 s2 D.
     move=>/andP[/eqP? bB]; subst => ssaB/=.
-    move=>/and3P[VA' VB']/andP[ssB0 bB0].
-    case NB' : (next_alt_aux true s1 B') => [[s3 E]|].
+    move=>/and3P[VA' VB'] bB0.
+    case NB' : (next_alt s1 B') => [[s3 E]|].
+      case:ifP => //.
       move=>[]??;subst.
-      rewrite (HB _ _ _ _ _ bB ssaB (valid_state_compose_and VB' bB0) NB')//.
+      rewrite (HB _ _ _ _ _ ssaB (valid_state_compose_and VB' bB0) NB')//.
       (* by rewrite (HB _ _ _ _ _ bB _ ssaB NB')./ *)
-    case NA' : (next_alt_aux true s1 A') => // [[s3 E]].
+    case NA' : (next_alt s1 A') => // [[s3 E]].
     move=>[]??;subst.
     move: VB'.
     case: ifP.
@@ -724,58 +668,62 @@ Module valid_state (U:Unif).
       apply: xxx ssaB ssB0 => //.
       (* admit. *)
     move=> _.
-    move=>/orP[]/eqP?;subst => //.
-    apply: ssa_cut2 => //.
-  Qed.
+    move=>/eqP?;subst => //.
+    (* apply: ssa_cut2 => //. *)
+  Qed. *)
 
-  Lemma valid_state_next_alt_aux {b s1 s2 A B}: 
-    valid_state A -> next_alt_aux b s1 A = Some (s2, B) 
+  Lemma valid_state_next_alt {s1 s2 A B}: 
+    valid_state A -> next_alt s1 A = Some (s2, B) 
     -> valid_state B.
   Proof.
-    elim: A b s1 s2 B => //.
+    elim: A s1 s2 B => //.
+    (* + by move=> [] // ??? _ [] /[subst2].
     + by move=> [] // ??? _ [] /[subst2].
-    + by move=> [] // ??? _ [] /[subst2].
-    + by move=> ?? [] // ??? _ [] /[subst2].
-    + move=> A HA s B HB b s1 s2 C /simpl_valid_state_or [].
-      + move=> [] /[subst1] /HB {}HB /=.
-        case X: next_alt_aux => // [[s3 D]].
-        move: X => /HB {}HB; destruct D => // -[]/[subst2]//.
-      + move=> [] DA [] /[dup] VA /HA {}HA /[dup] VBa.
-        move=> /base_or_base_or_ko_valid /[dup] VB /HB{}HB /simpl_next_alt_aux_some [|[]].
-        + by move=> [B'[?[+]]] /[subst1] => /HB /= ->.
-        + by move=> [A'[_ [+]]] /[subst1] /HA /= ->; rewrite VB VBa; destruct A'.
-        + by move=> [_ [NA]] /[subst1] /=.
-    + move=> A HA B0 HB0 B HB b s1 s2 C /simpl_valid_state_and1 [VA [VB [ssaB0 bB0]]]/=.
-      case NB: next_alt_aux => [[s3 D]|].
-        move=> [] /[subst2] /=; rewrite VA bB0.
-        have VD:= (HB _ _ _ _ (valid_state_compose_and VB bB0) NB).
-        rewrite VD.
+    + by move=> ?? [] // ??? _ [] /[subst2]. *)
+    + move=> A HA s B HB s1 s2 C /simpl_valid_state_or [].
+        move=> [-> VB]/=; rewrite dead_dead_same eqxx.
+        case X: next_alt => // [[s3 D]].
+        move=>[]??;subst => /=.
+        rewrite dead_dead_same eqxx; apply: HB VB X.
+      move=> [dA [VA bB]]/=.
+      case: ifP=>/eqP.
+        move=>->.
+        case X: next_alt => //[[s3 D]].
+        move=> []*;subst=>/=.
+        rewrite dead_dead_same eqxx.
+        apply: HB (base_or_base_or_ko_valid bB) X.
+      move=> _; case: ifP => /eqP// dB.
+      have VB:= base_or_base_or_ko_valid bB.
+      case X: next_alt => //[[s3 D]|].
+        move =>-[]*;subst=>/=.
+        by rewrite bB VB (HA _ _ _ VA X) if_same.
+      case:ifP => //.
+        case Y: next_alt => //[[s3 D]] fB []??;subst=> /=.
+        rewrite dead_dead_same eqxx.
+        by apply: HB Y.
+      move=> _ []??;subst => /=.
+      by rewrite dead_dead_same eqxx VB.
+    + move=> A HA B0 HB0 B HB s1 s2 C /simpl_valid_state_and1 [VA [VB bB0]]/=.
+      have VB' := valid_state_compose_and VB bB0.
+      case: ifP => ///eqP dA.
+      case: ifP => // fA.
+        case NA: next_alt => [[s3 D]|]//.
+        case: ifP => //fB0 []??;subst => /=.
+        rewrite bB0 eqxx (base_and_valid bB0) if_same !andbT.
+        apply: HA VA NA.
+      have N := @next_alt_aux_base_and1 B0 s1 bB0.
+      case NB: next_alt => // [[s3 D]|].
+        move=>[]??;subst => /=.
+        rewrite VA bB0 andbT/=.
         move: VB.
-        case: ifP => SA.
-          move=>VB.
-          have:= (ssa_next_alt_aux bB0 ssaB0 VB NB).
-          by move=>->.
-          (* by have:= next_alt_aux_base_and1 bB0 NB=>->; rewrite eqxx. *)
-        move=>/orP[]/eqP?;subst.
-          have ?:= (next_alt_aux_base_and1 bB0 NB); subst.
-          by rewrite ssaB0 eqxx.
-        have ?:= (next_alt_aux_base_and2 bB0 NB); subst.
-        by rewrite eqxx orbT (ssa_cut bB0).
-        (* by have:= next_alt_aux_base_and2 bB0 NB=>->; rewrite eqxx orbT. *)
-      case NA: next_alt_aux => // [[s3 D]] [] /[subst2] /=.
-      by rewrite (HA _ _ _ _ VA NA) eqxx bB0 (base_and_valid bB0) if_same ssa_id.
-  Qed.
-
-  Lemma valid_state_next_alt {s s' A B} : 
-    next_alt s A (Some (s', B)) -> valid_state A ->  valid_state B.
-  Proof.
-    remember (Some _) as S eqn:HS.
-    move=> H; elim: H s' B HS => //; clear.
-    + move=> s s2 A B' + FA s1 B [] /[subst2].
-      by move=> /valid_state_next_alt_aux H1.
-    + move=> s s1 r A B NA FB NB IH s2 D /[subst1] VA.
-      have VB:= valid_state_next_alt_aux VA NA.
-      apply: IH erefl VB.
+        case: ifP => // sA.
+          move=> vB.
+          apply: HB VB' NB.
+        move=>/eqP?;subst.
+        congruence.
+      case NA: next_alt => //[[s3 D]].
+      case: ifP => // _ []??;subst => /=.
+      by rewrite (HA _ _ _ VA NA) eqxx bB0 (base_and_valid bB0) if_same.
   Qed.
 
   Lemma runP_run {s A r}:
@@ -789,8 +737,76 @@ Module valid_state (U:Unif).
       apply: valid_state_expanded VA (ex_intro _ _ HA).
     + move=> s s' r A B C b1 b2 b3 HA HB HC IH Hb VA.
       have VB := valid_state_expanded VA (ex_intro _ _ HA).
-      have NA := valid_state_next_alt HB VB.
+      have NA := valid_state_next_alt VB HB.
       apply: IH NA.
     Qed.
+
+  Lemma base_and_ko_succes {B}: base_and_ko B -> success B = false.
+  Proof. elim: B => // -[]//=. Qed.
+
+  Lemma base_and_succes {B}: base_and B -> success B = false.
+  Proof. elim: B => // -[]//=. Qed.
+
+  Lemma base_or_succes {B}: base_or_aux B || base_or_aux_ko B -> success B = false.
+  Proof.
+    move=>/orP[].
+      elim: B => //.
+        move=> A HA s B HB/=/andP[].
+        case: ifP=>/eqP.
+          by move=>->; rewrite base_and_dead.
+        by move=> dA /base_and_succes.
+      move=> []//.
+    elim: B=> //=.
+      move=> A HA _ B HB/andP[].
+      case: ifP=>/eqP//.
+      by move=> _ /base_and_ko_succes.
+    move=> []//.
+  Qed.
+
+  Lemma next_alt_aux_success {A B s1 s2}: valid_state A -> next_alt s1 A = Some (s2, B) -> success B = false.
+  Proof.
+    elim: A B s1 s2 => //.
+      move=> A HA s B HB B0 s1 s2/simpl_valid_state_or[].
+        move=>[-> VB]/=; rewrite dead_dead_same eqxx.
+        have:= HB _ s1 _ VB.
+        case X: next_alt => //[[s3 C]] => /(_ _ _ erefl).
+        move=> _ []??;subst => /=.
+        rewrite dead_dead_same eqxx.
+        apply: HB VB X.
+      move=> [dA [VA VB]]/=; case: ifP => /eqP// _.
+      case: ifP => ///eqP dB.
+      have:= HA _ s1 _ VA.
+      case: next_alt => [[s3 C]|].
+        move=>/(_ _ _ erefl) + []??; subst => /=.
+        case: ifP => ///eqP.
+        by rewrite (base_or_succes VB).
+      have VB':= base_or_base_or_ko_valid VB.
+      case:ifP => // fB _.
+        case X: next_alt => //[[s3 C]].
+        move=> []??;subst => /=.
+        rewrite dead_dead_same eqxx.
+        by apply: HB X.
+      move=> []??;subst => /=.
+      rewrite dead_dead_same eqxx.
+      by apply: base_or_succes.
+    move=> A HA B0 _ B HB B1 s1 s2 /simpl_valid_state_and1[VA [VB bB0]].
+    move=>/=.
+    case:ifP => ///eqP dA.
+    case: ifP => //fA.
+      case: next_alt => //[[s3 C]].
+      case: ifP => //fB0.
+      move=> []??;subst => /=.
+      by rewrite (base_and_succes bB0) andbF.
+    have:= HB _ s1 _ (valid_state_compose_and VB bB0).
+    case: next_alt => [[s3 C]|].
+      by move=>/(_ _ _ erefl) + []??;subst => /= ->; rewrite andbF.
+    move=> _.
+    have:= HA _ s1 _ VA.
+    case: next_alt => [[s3 C]|]// /(_ _ _ erefl).
+    case:ifP => //.
+    move=> _ + []??; subst.
+    by move=>/=->.
+  Qed.
+
 
 End valid_state.
